%iffalse
\let\negmedspace\undefined
\let\negthickspace\undefined
\documentclass[journal,12pt,twocolumn]{IEEEtran}
\usepackage{cite}
\usepackage{amsmath,amssymb,amsfonts,amsthm}
\usepackage{algorithmic}
\usepackage{graphicx}
\usepackage{textcomp}
\usepackage{xcolor}
\usepackage{txfonts}
\usepackage{listings}
\usepackage{enumitem}
\usepackage{mathtools}
\usepackage{gensymb}
\usepackage{comment}
\usepackage[breaklinks=true]{hyperref}
\usepackage{tkz-euclide} 
\usepackage{listings}
\usepackage{gvv}                                        
%\def\inputGnumericTable{}                                 
\usepackage[latin1]{inputenc}                                
\usepackage{color}                                            
\usepackage{array}                                            
\usepackage{longtable}                                       
\usepackage{calc}                                             
\usepackage{multirow}                                         
\usepackage{hhline}                                           
\usepackage{ifthen}                                           
\usepackage{lscape}
\usepackage{tabularx}
\usepackage{array}
\usepackage{float}


\newtheorem{theorem}{Theorem}[section]
\newtheorem{problem}{Problem}
\newtheorem{proposition}{Proposition}[section]
\newtheorem{lemma}{Lemma}[section]
\newtheorem{corollary}[theorem]{Corollary}
\newtheorem{example}{Example}[section]
\newtheorem{definition}[problem]{Definition}
\newcommand{\BEQA}{\begin{eqnarray}}
\newcommand{\EEQA}{\end{eqnarray}}
\newcommand{\define}{\stackrel{\triangle}{=}}
\theoremstyle{remark}
\newtheorem{rem}{Remark}

% Marks the beginning of the document
\begin{document}
\bibliographystyle{IEEEtran}
\vspace{3cm}

\title{JEE Chapter 19 CD}
\author{AI24BTECH11028 - Ronit Ranjan}
\maketitle
\newpage
\bigskip
\section*{C. MCQ with one correct answer}

1. A solution of the differential equation \hfill (1999 - 2 Marks)
\[
\brak{\frac{dy}{dx}}^2 - x \frac{dy}{dx} + y = 0 \text{ is}
\]
\begin{enumerate}[label=(\alph*)]
    \item $y = 2$ \quad \quad \quad \quad (b) $y = 2x$
    \item $y = 2x - 4$ \quad \quad (d) $y = 2x^2 - 4$
\end{enumerate}

2. If $x^2 + y^2 = 1$, then \hfill (2000S)
\begin{enumerate}[label=(\alph*)]
    \item $yy'' - 2\brak{y'}^2 + 1 = 0$ \quad \quad (b) $yy'' + \brak{y'}^2 + 1 = 0$
    \item $yy'' + \brak{y'}^2 - 1 = 0$ \quad (d) $yy'' + 2\brak{y'}^2 + 1 = 0$
\end{enumerate}

3. If $y\brak{t}$ is a solution of $\brak{1 + t} \frac{dy}{dt} - ty = 1$ and $y\brak{0} = -1$, then \hfill (2003S)
\[
y\brak{1} \text{ is equal to}
\]
\begin{enumerate}[label=(\alph*)]
    \item $-\frac{1}{2}$ \quad \quad \quad \quad (b) $e + \frac{1}{2}$
    \item $e - \frac{1}{2}$ \quad \quad \quad (d) $\frac{1}{2}$
\end{enumerate}

4. If $y = y\brak{x}$ and $\frac{2 + \sin x}{y + 1}\brak{\frac{dy}{dx}} = -\cos x$, $y\brak{0} = 1$, then y\brak{\frac{\pi}{2}} \hfill (2004S)

\begin{enumerate}[label=(\alph*)]
    \item $\frac{1}{3}$ \quad \quad \quad (b) $\frac{2}{3}$
    \item $-\frac{1}{3}$ \quad \quad (d) $1$
\end{enumerate}
5. If $y = y(x)$ and it follows the relation $x \cos y + y \cos x = \pi$ then $y''(0) =$ \hfill (2005S)
\begin{enumerate}[label=(\alph*)]
    \item $1$ \quad \quad \quad (b) $-1$
    \item $\pi - 1$ \quad \quad (d) $-\pi$
\end{enumerate}

6. The solution of primitive integral equation $\brak{x^2 + y^2}dy = xy \, dx$ is $y = y(x)$. If $y(1) = 1$ and $x_0 = e$, then $x_0$ is equal to \hfill (2005S)
\begin{enumerate}[label=(\alph*)]
    \item $\sqrt{2\brak{e^2 - 1}}$ \quad (b) $\sqrt{2\brak{e^2 + 1}}$
    \item $\sqrt{3e}$ \quad \quad \quad (d) $\sqrt{\frac{e^2 + 1}{2}}$
\end{enumerate}

7. For the primitive integral equation $y dx + y^2 dy = x \, dy$; $x \in \mathbb{R}, y > 0, y = y(x), y(1) = 1$, then $y(-3)$ is \hfill (2005S)
\begin{enumerate}[label=(\alph*)]
    \item $3$ \quad \quad \quad \quad (b) $2$
    \item $1$ \quad \quad \quad \quad (d) $5$
\end{enumerate}

8. The differential equation $\frac{dy}{dx} = \frac{\sqrt{1-y^2}}{y}$ determines a family of circles with \hfill (2005S)
\begin{enumerate}[label=(\alph*)]
    \item [(a)] variable radii and a fixed centre at \brak{0,1}
    \item [(b)] variable radii and a fixed centre at \brak{0, -1}
    \item [(c)] fixed radius 1 and variable centres along the x-axis
    \item [(d)] fixed radius 1 and variable centres along the y-axis
\end{enumerate}
9. The function $y = f(x)$ is the solution of the differential equation
\[
\frac{dy}{dx} + \frac{xy}{x^2-1} = \frac{x^4 + 2x}{\sqrt{1-x^2}}
\]
in $(-1, 1)$ satisfying $f(0) = 0$. Then
\[
\int_{-\frac{\sqrt{3}}{2}}^{\frac{\sqrt{3}}{2}} f(x) \, dx \text{ is}
\]
\begin{enumerate}[label=(\alph*)]
    \item $\frac{\pi}{3} - \frac{\sqrt{3}}{2}$ \quad (b) $\frac{\pi}{3} - \frac{\sqrt{3}}{4}$
    \item $\frac{\pi}{6} - \frac{\sqrt{3}}{4}$ \quad (d)$\frac{\pi}{6} - \frac{\sqrt{3}}{2}$
\end{enumerate}

10. If $y = y(x)$ satisfies the differential equation
\[
8\sqrt{x} \brak{\sqrt{9+\sqrt{x}}} dy = \brak{\sqrt{4+\sqrt{9+\sqrt{x}}}}^{-1} dx, \, x>0 \text{ and}
\]

y(0) = $\sqrt{7}$, \text{ then } y(256) = 
\begin{enumerate}[label=(\alph*)]
    \item 3 \quad\quad\quad (b) 9
    \item 16\quad\quad\quad (d) 80
\end{enumerate}
\section*{D. MCQ with one or more than correct answer}

1. The order of the differential equation whose general solution is given by
$y = \brak{C_1 + C_2} \cos \brak{x + C_3} - C_4 e^{x+C_5}$, where $C_1, C_2, C_3, C_4, C_5$ are arbitrary constants, is \hfill (1998 - 2 Marks)

\begin{enumerate}[label=(\alph*)]
    \item 5 \quad\quad\quad (b) 4
    \item 3 \quad\quad\quad (d) 2
\end{enumerate}


2. The differential equation representing the family of curves
$y^2 = 2c \brak{x + \sqrt{c}}$, where c  is a positive parameter, is of \hfill(1999 - 3 Marks)
\begin{enumerate}[label=(\alph*)]
    \item order 1 \quad\quad  (b)order 2
    \item degree 3 \quad (d)degree 4
\end{enumerate}

3. A curve \( y = f(x) \) passes through \( \brak{1,1} \) and at \( P\brak{x, y} \), the tangent cuts the \( x \)-axis and \( y \)-axis at \( A \) and \( B \) respectively such that \( BP : AP = 3 : 1 \), then
\begin{enumerate}[label=(\alph*)]
    \item equation of curve is \( xy' - 3y = 0 \)
    \item normal at \( \brak{1, 1} \) is \( x + 3y = 4 \)
    \item curve passes through \( \brak{2, \frac{1}{8}} \)
    \item equation of curve is \( xy' + 3y = 0 \)
\end{enumerate}

4. If \( y\brak{x} \) satisfies the differential equation \( y' - y \tan x = 2x \sec x \) and \( y\brak{0} = 0 \), then
\begin{enumerate}[label=(\alph*)]
    \item \( y\brak{\frac{\pi}{4}} = \frac{\pi^2}{8\sqrt{2}} \) \quad (b) \( y\brak{\frac{\pi}{4}} = \frac{\pi^2}{18} \) 
    \item \( y\brak{\frac{\pi}{3}} = \frac{\pi^2}{9} \) \quad \quad (d) \( y\brak{\frac{\pi}{3}} = \frac{4\pi}{3} + \frac{2\pi^2}{3\sqrt{3}} \)
\end{enumerate}

5. A curve passes through the point \( \brak{1,\frac{\pi}{6}} \). Let the slope of the curve at each point \( \brak{x, y} \) be \( \frac{y}{x} + \sec\brak{\frac{y}{x}}, x > 0 \). Then the equation of the curve is 
\begin{enumerate}[label=(\alph*)]
    \item \( \sin\brak{\frac{y}{x}} = \log x + \frac{1}{2} \) \quad(b) \( \cos\sec\brak{\frac{y}{x}} = \log x + 2 \) 
    \item \( \sec\brak{\frac{2y}{x}} = \log x + 2 \) \quad (d) \( \cos\brak{\frac{2y}{x}} = \log x + \frac{1}{2} \)
\end{enumerate}

\end{document}
